toCNF function + proof of correspondence via eval; + cleanups

Solver.thy
@@ -1,5 +1,5 @@
 theory Solver
-  imports Main
+  imports Main 
 begin
 
 datatype formula = Var string | Const bool | Not formula | And formula formula | Or formula formula
@@ -42,14 +42,13 @@ fun leval :: "literal \<Rightarrow> state \<Rightarrow> bool"
 
 fun ceval :: "clauseCNF \<Rightarrow> state \<Rightarrow> bool"
   where
-    "ceval [] s = True"
+    "ceval [] s = False"
   | "ceval (l # ls) s = (leval l s \<or> ceval ls s)"
 
 fun evalCNF :: "formulaCNF \<Rightarrow> state \<Rightarrow> bool"
   where
-    "evalCNF [] s = False"
-  | "evalCNF [c] s = ceval c s"
-  | "evalCNF (c # c' # cs) s = (ceval c s \<and> evalCNF (c' # cs) s)"
+    "evalCNF [] s = True"
+  | "evalCNF (c # cs) s = (ceval c s \<and> evalCNF cs s)"
 
 fun literal_to_formula :: "literal \<Rightarrow> formula"
   where
@@ -58,33 +57,71 @@ fun literal_to_formula :: "literal \<Rightarrow> formula"
 
 fun clause_to_formula :: "clauseCNF \<Rightarrow> formula"
   where
-    "clause_to_formula [] = Const True"
+    "clause_to_formula [] = Const False"
   | "clause_to_formula (l # ls) = Or (literal_to_formula l) (clause_to_formula ls)"
 
-fun cnf_to_formula :: "formulaCNF \<Rightarrow> formula"
+fun toFormula :: "formulaCNF \<Rightarrow> formula"
   where
-    "cnf_to_formula [] = Const False"
-  | "cnf_to_formula [c] = (if c = [] then Const True else clause_to_formula c)"
-  | "cnf_to_formula (c#cs) = And (clause_to_formula c) (cnf_to_formula cs)"
+    "toFormula [] = Const True"
+  | "toFormula (c # cs) = And (clause_to_formula c) (toFormula cs)"
 
 
-thm "list.induct"
-
-lemma "Q [] \<Longrightarrow> (\<And>x. Q [x]) \<Longrightarrow> (\<And>x y xs. Q xs \<Longrightarrow> Q (y # xs) \<Longrightarrow> Q (x # y # xs)) \<Longrightarrow> Q xs"
-  sorry
-
-lemma ltf_correct: "leval l s \<longleftrightarrow> eval (literal_to_formula l) s"
+lemma ltf_eval: "leval l s \<longleftrightarrow> eval (literal_to_formula l) s"
   by (induction l) auto
 
-lemma ctf_correct: "ceval c s \<longleftrightarrow> eval (clause_to_formula c) s"
-  apply (induction c)
-   apply (auto simp: ltf_correct)
-  done
+lemma ctf_eval: "ceval c s \<longleftrightarrow> eval (clause_to_formula c) s"
+  by (induction c) (auto simp: ltf_eval)
 
-lemma conv_correct: "evalCNF cs s \<longleftrightarrow> eval (cnf_to_formula cs) s"
-  apply (induction cs rule: induct_list012)
-  apply (auto simp: ctf_correct)
-  done
+lemma toFormula_eval: "evalCNF cs s \<longleftrightarrow> eval (toFormula cs) s"
+  by (induction cs) (auto simp: ctf_eval)
+
+fun toCNF :: "formula \<Rightarrow> formulaCNF"
+  where
+    "toCNF (Var x) = [[P x]]"
+  | "toCNF (Const b) = (if b then [] else [[]])"
+(*| "toCNF (Not F) = (case F of (Var x) \<Rightarrow> [[N x]] 
+                                | Const b \<Rightarrow> toCNF (Const (\<not>b)) 
+                                | Not G \<Rightarrow> toCNF G
+                                | And G H \<Rightarrow> [c1@c2 . c1 \<leftarrow> toCNF (Not G), c2 \<leftarrow> toCNF (Not H)]
+                                | Or G H \<Rightarrow> toCNF (Not G) @ toCNF (Not H))"*)
+  | "toCNF (Not (Var x)) = [[N x]]"
+  | "toCNF (Not (Const b)) = toCNF (Const (\<not>b))"
+  | "toCNF (Not (Not G)) = toCNF G"
+  | "toCNF (Not (And F G)) = [c1@c2 . c1 \<leftarrow> toCNF (Not F), c2 \<leftarrow> toCNF (Not G)]"
+  | "toCNF (Not (Or F G)) = toCNF (Not F) @ toCNF (Not G)"
+  | "toCNF (And F G) = (toCNF F) @ (toCNF G)"
+  | "toCNF (Or F G) = [c1@c2 . c1 \<leftarrow> toCNF F, c2 \<leftarrow> toCNF G]"
 
 
+lemma evalCNF_app: "evalCNF (cs1 @ cs2) s = (evalCNF cs1 s \<and> evalCNF cs2 s)"
+  by (induction cs1) auto
+
+lemma evalCNF_fold_aux: "(b \<and> evalCNF cs s) = fold (\<lambda>c b. ceval c s \<and> b) cs b"
+  by (induction cs arbitrary: b) (simp_all, metis)
+
+lemma evalCNF_is_fold: "evalCNF cs s = fold (\<lambda>c b. ceval c s \<and> b) cs True"
+  using evalCNF_fold_aux by auto
+
+lemma ceval_app: "ceval (c1 @ c2) s = (ceval c1 s \<or> ceval c2 s)"
+  by (induction c1) auto
+
+
+lemma cnf_or_distr: "evalCNF (map ((@) a) cs) s = (ceval a s \<or> evalCNF cs s)"
+  by (induction cs) (auto simp: ceval_app)
+
+lemma cnf_or: "evalCNF [c1@c2 . c1 \<leftarrow> cs1, c2 \<leftarrow> cs2] s = (evalCNF cs1 s \<or> evalCNF cs2 s)"
+  by (induction cs1) (auto simp: evalCNF_app cnf_or_distr)
+  
+lemma deMorgan_NAND: "eval (Not (And F G)) = eval (Or (Not F) (Not G))"
+  by (induction F) auto
+
+lemma deMorgan_NOR: "eval (Not (Or F G)) = eval (And (Not F) (Not G))"
+  by (induction F) auto
+
+lemma evalCNF_not: "evalCNF (toCNF (formula.Not F)) s = (\<not>evalCNF (toCNF F) s)"
+  by (induction F) (auto split: if_splits simp: evalCNF_app cnf_or)
+
+lemma toCNF_eval: "eval F s \<longleftrightarrow> evalCNF (toCNF F) s"
+  by (induction F) (auto simp: evalCNF_app cnf_or evalCNF_not)
+  
 end
